theories/Substitution/Reduction.v
@@ -14,25 +14,11 @@ Lemma redwfSubstValid {Γ A t u l}
   (red : [Γ ||-v t :⤳*: u : A | VΓ])
   (VA : [Γ ||-v<l> A | VΓ])
   (Vu : [Γ ||-v<l> u : A | VΓ | VA]) :
-  [Γ ||-v<l> t : A | VΓ | VA] × [Γ ||-v<l> t ≅ u : A | VΓ | VA].
+  [Γ ||-v<l> t ≅ u : A | VΓ | VA].
 Proof.
-  assert (Veq : [Γ ||-v<l> t ≅ u : A | VΓ | VA]).
-  {
-    constructor; intros; eapply redwfSubstTerm.
-    1: now eapply validTm.
-    now eapply validRed.
-  }
-  split; tea; constructor; intros.
-  - eapply redwfSubstTerm.
-    1: now eapply validTm.
-    now eapply validRed.
-  - eapply transEqTerm. 2: eapply transEqTerm.
-    + now eapply validTmEq.
-    + now eapply validTmExt.
-    + eapply LRTmEqSym. eapply LRTmEqRedConv.
-      1: eapply LRTyEqSym; now eapply validTyExt.
-      now eapply validTmEq.
-      Unshelve. all: tea.
+  constructor; intros. eapply redwfSubstTmEq.
+  1: now eapply validTmExt.
+  now eapply validRed.
 Qed.
-   
+
 End Reduction.
