theories/Substitution/Reflexivity.v
@@ -1,6 +1,7 @@
 From LogRel.AutoSubst Require Import core unscoped Ast Extra.
 From LogRel Require Import Utils BasicAst Notations Context NormalForms Weakening GenericTyping LogicalRelation Validity.
-From LogRel.LogicalRelation Require Import Irrelevance Escape Reflexivity Weakening Neutral.
+From LogRel.LogicalRelation Require Import Irrelevance EqRedRight.
+From LogRel.Substitution Require Import Irrelevance Properties.
 
 Set Universe Polymorphism.
 
@@ -11,7 +12,21 @@ Lemma reflValidTy {Γ A l} (VΓ : [||-v Γ])
   (VA : [Γ ||-v<l> A | VΓ]) :
   [Γ ||-v<l> A ≅ A | VΓ | VA].
 Proof.
-  constructor; intros; apply reflLRTyEq.
+  constructor; intros; eapply validTyExt.
+Qed.
+Set Printing Primitive Projection Parameters.
+
+Lemma ureflValidTy {Γ A B l} (VΓ : [||-v Γ])
+  (VA : [Γ ||-v<l> A | VΓ])
+  (VAB : [Γ ||-v<l> A ≅ B | VΓ | VA]) :
+  [Γ ||-v<l> B | VΓ ].
+Proof.
+  unshelve econstructor; intros.
+  1: (unshelve now eapply LRTyEqRedRight, validTyEq); [tea| |now eapply lrefl].
+  eapply LRTransEq.
+  2: (unshelve now eapply validTyEq); cycle 2; tea.
+  eapply LRTyEqSym.
+  (unshelve now eapply validTyEq); tea; now eapply lrefl.
 Qed.
 
 Lemma reflValidTm {Γ t A l} (VΓ : [||-v Γ])
@@ -19,7 +34,29 @@ Lemma reflValidTm {Γ t A l} (VΓ : [||-v Γ])
   (Vt : [Γ ||-v<l> t : A | VΓ | VA]) :
   [Γ ||-v<l> t ≅ t : A | VΓ | VA].
 Proof.
-  constructor; intros; apply reflLRTmEq; now eapply validTm.
+  constructor; intros; now eapply validTmExt.
+Qed.
+
+Lemma lreflValidTm {Γ t u A l} (VΓ : [||-v Γ])
+  (VA : [Γ ||-v<l> A | VΓ])
+  (Vtu : [Γ ||-v<l> t ≅ u : A | VΓ | VA]) :
+  [Γ ||-v<l> t : A | VΓ | VA].
+Proof.
+  constructor; intros.
+  etransitivity; [now eapply validTmEq|symmetry].
+  eapply LRTmEqConv.
+  2: now eapply validTmEq.
+  eapply LRTyEqSym.
+  eapply validTyExt.
+  Unshelve. 1,6-8:tea. now eapply urefl.
+Qed.
+
+Lemma ureflValidTm {Γ t u A l} (VΓ : [||-v Γ])
+  (VA : [Γ ||-v<l> A | VΓ])
+  (Vtu : [Γ ||-v<l> t ≅ u : A | VΓ | VA]) :
+  [Γ ||-v<l> u : A | VΓ | VA].
+Proof.
+  eapply lreflValidTm; now eapply symValidTmEq.
 Qed.
 
 End Reflexivity.
